theories/STB.v
@@ -6,7 +6,6 @@ Require Import ModSem.
 Require Import Skeleton.
 Require Import PCM.
 Require Import HoareDef.
-Require Import TODOYJ.
 Require Import Logic.
 
 Generalizable Variables E R A B C X Y Σ.
@@ -18,7 +17,48 @@ Section HEADER.
 
   Context `{Σ: GRA.t}.
 
+  Definition ftspec_weaker Y Z (fsp_src fsp_tgt: ftspec Y Z): Prop :=
+    forall (x_src: fsp_src.(X)),
+    exists (x_tgt: fsp_tgt.(X)),
+      (<<PRE: forall arg_src arg_tgt o,
+          (fsp_src.(precond) x_src arg_src arg_tgt o -* fsp_tgt.(precond) x_tgt arg_src arg_tgt o) ε>>) /\
+      (<<POST: forall ret_src ret_tgt,
+          (fsp_tgt.(postcond) x_tgt ret_src ret_tgt -* fsp_src.(postcond) x_src ret_src ret_tgt) ε>>)
+  .
 
+  Global Program Instance ftspec_weaker_PreOrder Y Z: PreOrder (@ftspec_weaker Y Z).
+  Next Obligation.
+  Proof.
+    ii. exists x_src. esplits; ii.
+    { rewrite URA.unit_idl. auto. }
+    { rewrite URA.unit_idl. auto. }
+  Qed.
+  Next Obligation.
+  Proof.
+    ii. hexploit (H x_src). i. des.
+    hexploit (H0 x_tgt). i. des. esplits; ii.
+    { eapply PRE0; ss. rewrite <- URA.unit_idl. eapply PRE; auto. }
+    { eapply POST; ss. rewrite <- URA.unit_idl. eapply POST0; auto. }
+  Qed.
+
+  Variant fspec_weaker (fsp_src fsp_tgt: fspec): Prop :=
+  | fspec_weaker_intro
+      Y Z ftsp_src ftsp_tgt
+      (FSPEC0: fsp_src = @mk_fspec _ Y Z ftsp_src)
+      (FSPEC1: fsp_tgt = @mk_fspec _ Y Z ftsp_tgt)
+      (WEAK: ftspec_weaker ftsp_src ftsp_tgt)
+  .
+
+  Global Program Instance fspec_weaker_PreOrder: PreOrder fspec_weaker.
+  Next Obligation.
+  Proof.
+    ii. destruct x. econs; eauto. refl.
+  Qed.
+  Next Obligation.
+  Proof.
+    ii. inv H; inv H0. dependent destruction FSPEC0.
+    econs; eauto. etrans; eauto.
+  Qed.
 
   Variant fn_has_spec (stb: list (gname * fspec)) (fn: gname) Y Z (ftsp: ftspec Y Z): Prop :=
   | fn_has_spec_intro
