examples/knot/Knot01proof.v
@@ -1,4 +1,4 @@
-Require Import HoareDef KnotHeader Knot0 Knot1 SimModSemL SimModSem.
+Require Import HoareDef STB KnotHeader Knot0 Knot1 SimModSemL SimModSem.
 Require Import Coqlib.
 Require Import Universe.
 Require Import Skeleton.
@@ -115,23 +115,16 @@ Section SIMMODSEM.
         (<<TGT: mrps_tgt0 = (ε, fb'↑)>>) /\
         (<<SIM: (iHyp (Own (GRA.embed (knot_full f'))) mr)>>) /\
         (<<SOME: forall f (FUN: f' = Some f),
-            exists fb fn,
+            exists fb,
               (<<BLK: fb' = Some fb>>) /\
-              (<<FN: skenv.(SkEnv.blk2id) fb = Some fn>>) /\
-              (<<FIND: List.find (fun '(_fn, _) => dec fn _fn) (FunStb skenv) = Some (fn, mk_fspec (fun_gen RecStb skenv f))>>)>>)
+              (<<FN: fb_has_spec skenv (FunStb skenv) fb (fun_gen RecStb skenv f)>>)>>)
   .
 
-  Variable RecStb_incl
-    :
-      forall skenv fn fsp
-             (SPECS: List.find (fun '(_fn, _) => dec fn _fn) KnotRecStb = Some fsp),
-        List.find (fun '(_fn, _) => dec fn _fn) (RecStb skenv) = Some fsp.
+  Hypothesis RecStb_incl: forall skenv,
+      stb_incl KnotRecStb (RecStb skenv).
 
-  Variable FunStb_incl
-    :
-      forall skenv fn fsp
-             (SPECS: List.find (fun '(_fn, _) => dec fn _fn) (FunStb skenv) = Some fsp),
-        List.find (fun '(_fn, _) => dec fn _fn) (GlobalStb skenv) = Some fsp.
+  Hypothesis FunStb_incl: forall skenv,
+      stb_incl (FunStb skenv) (GlobalStb skenv).
 
   Variable MemStb_incl
     :
@@ -168,15 +161,20 @@ Section SIMMODSEM.
       assert (f' = Some f); subst.
       { hexploit knot_ra_merge; et. intro T. iSpecialize T SIM. iSpecialize T PRE. iPure T. auto. }
       hexploit SOME; eauto. clear SOME. i. des. clarify. steps.
-      rewrite Any.upcast_downcast. ss. steps. rewrite FN. ss. steps.
+      rewrite Any.upcast_downcast. ss. steps.
+      dup FN. inv FN. rewrite FBLOCK. steps.
       hexploit (SKINCL "rec"); ss; eauto. i. des. rewrite H0. ss. steps.
-      acall_tac_weaken (fun_gen RecStb skenv f) n (ord_pure (2 * n)) SIM (@URA.unit Σ) PRE.
-      { eapply FunStb_incl. eapply FIND. }
-      { refl. }
+      inv SPEC. exploit FunStb_incl; et. i.
+      acatch.
+      { eapply x1. }
+      hcall_tac_weaken (fun_gen RecStb skenv f) n (ord_pure (2 * n)) SIM (@URA.unit Σ) PRE.
+      { et. }
       { ss. splits; ss. iRefresh. iSplitR PRE; ss.
-        red. red. esplits; eauto.
+        red. red. esplits; eauto. econs; eauto.
         { eapply SKWF. eauto. }
+        econs.
         { eapply RecStb_incl. des_ifs. }
+        { refl. }
       }
       { splits; ss. eauto with ord_step. }
       { ss. esplits; eauto. i. clarify. esplits; eauto. }
@@ -201,32 +199,17 @@ Section SIMMODSEM.
         instantiate (1:= knot_full (Some x) ⋅ knot_frag (Some x)).
         eapply Auth.auth_update. rr. ii. des; ss. ur in FRAME. ur. destruct ctx; ss; clarify.
       }
-      rewrite <- GRA.embed_add in SEP. rewrite own_sep in SEP. iDestruct SEP.
-      steps. rewrite FIND1. steps.
-      iDestruct A0. iDestruct A0. iPure A1.
-      acall_tac (blk1, 0%Z, Vptr fb 0) (ord_pure 0) A SEP A0; ss.
-      { eapply MemStb_incl. stb_tac. ss. }
-      { splits; ss. iRefresh. iExists x5. iSplitL A0; ss.
-        iSplitR A0; ss. unfold knot_var in *. rewrite FIND1 in *. iApply A0. }
-      { splits; ss. eauto with ord_step. }
-      { esplits; eauto. iLeft. iApply A. }
-      steps. ss. des; clarify.
-      rewrite Any.upcast_downcast in _UNWRAPN. clarify. iDestruct SEP0; cycle 1.
-      { iDestruct SEP0. iExploitP (@knot_full_unique _ _ f'0 (Some x)); ss. }
-      iExploitP (@knot_ra_merge _ _ (Some x) f'0). i. subst.
-      astop. rewrite FIND0. steps. force_l. eexists.
-      iMerge POST SEP. hret_tac POST SEP0; ss.
-      { esplits; eauto. iRefresh. iSplitR SEP0; ss. red. red. esplits; eauto.
+      rewrite <- GRA.embed_add in SIM. rewrite own_sep in SIM. iDestruct SIM.
+      force_l. eexists.
+      hret_tac SIM A; ss.
+      { esplits; eauto. iRefresh. iSplitR A; eauto. red. red. esplits; eauto.
+        econs; eauto.
         { eapply SKWF; eauto. }
-        { eapply RecStb_incl; eauto. }
+        econs.
+        { eapply RecStb_incl; eauto. ss. }
+        { refl. }
       }
-      { iDestruct POST. esplits; eauto. iRight. iSplitL A; ss.
-        { iApply A. }
-        { iExists (Vptr fb 0). iSplitL POST.
-          { unfold knot_var. rewrite FIND1. iApply POST. }
-          { red. red. i. clarify. esplits; eauto. }
-        }
-      }
+      { esplits; eauto. i. clarify. esplits; eauto. }
     }
   Qed.
 
